theories/rules/rules_Get.v
@@ -139,7 +139,7 @@ Section cap_lang_rules.
   Qed.
 
 
-  Lemma wp_Get pc_p pc_b pc_e pc_a pc_v lw get_i dst src regs :
+  Lemma wp_Get Ep pc_p pc_b pc_e pc_a pc_v lw get_i dst src regs :
     decodeInstrWL lw = get_i →
     is_Get get_i dst src →
 
@@ -149,7 +149,7 @@ Section cap_lang_rules.
 
     {{{ ▷ (pc_a, pc_v) ↦ₐ lw ∗
         ▷ [∗ map] k↦y ∈ regs, k ↦ᵣ y }}}
-      Instr Executable @ ∅
+      Instr Executable @ Ep
     {{{ regs' retv, RET retv;
         ⌜ Get_spec (decodeInstrWL lw) regs dst src regs' retv ⌝ ∗
         (pc_a, pc_v) ↦ₐ lw ∗
